theories/Universe.v
@@ -9,10 +9,7 @@ Context `{Universe}.
 Inductive event: Type :=
 | event_sys
     (sys: syscall)
-| event_exit (rv: val)
 (* | event_tau *)
-| event_ub
-| event_nb
 .
 
 (* Coercion event_sys: syscall >-> event. *)
